\documentstyle[12pt]{article}
\usepackage{html}

\begin{document}


The canonical 2nd-order LCCODE 
\[
y''(t)+2\zeta\omega_n y(t)+\omega_n^2 y(t)=x(t)
\]
caan be converted into a 1st-order ODE system containing two 
1st-order LCCODEs (see 
\htmladdnormallink{here}{../../../e176/lectures/ch5/node9.html}):
\[
{\bf y}'=\left[\begin{array}{c}y_1'\\y_2'\end{array}\right]
=\left[\begin{array}{cc}0 & 1\\-\omega_n^2 & -2\zeta\omega_n\end{array}
\right]\left[\begin{array}{c}y_1\\y_2\end{array}\right]
+\left[\begin{array}{c}0\\x(t)\end{array}\right]
={\bf Ay}+{\bf x}
\]
The characteristic equation of the coefficient matrix ${\bf A}$ is
\[
\det(\lambda{\bf I}-{\bf A})
=\det\left[\begin{array}{cc}\lambda & -1\\\omega_n^2 & \lambda+2\zeta\omega_n
\end{array}\right]
=\lambda^2+2\zeta\omega_n\lambda+\omega_n^2=0
\]
Solving which we get the two eigenvalues and the eigenvalue matrix:
\[
\lambda_{1,2}=(-\zeta\pm\sqrt{\zeta^2-1})\omega_n
\;\;\;\;\;\;\;
{\bf\Lambda}=\left[\begin{array}{cc}\lambda_1 & 0\\0 & \lambda_2\end{array}\right]
\]
Note that
\[
\lambda_1\lambda_2=\omega_n^2,\;\;\;\;\;\;\;\;\;\;
\lambda_2-\lambda_1=2\omega_n\sqrt{\zeta^2-1}
\]

The eigenvector matrix and its inverse are:
\[
{\bf V}=\left[\begin{array}{cc}1 & 1\\ \lambda_1 & \lambda_2\end{array}\right],
\;\;\;\;\;\;
{\bf V}^{-1}=\frac{1}{\lambda_2-\lambda_1}
\left[\begin{array}{cc}\lambda_2 & -1\\ -\lambda_1 & 1\end{array}\right]
\]
and we can verify thatat ${\bf A}={\bf V\Lambda V}^{-1}$. 

\begin{itemize}
\item Homogeneous solution $x(t)=0$:

  Assuming $y_1(0)=y(0)=y_0$ and $y_2(0)=y'(0)=0$, we get the homogeneous 
  solution:

  \begin{eqnarray}
  {\bf y}_h(t)&=&e^{{\bf A}t}{\bf y}(0)={\bf V}e^{{\bf\Lambda}t}{\bf V}^{-1}{\bf y}(0)
  =\frac{1}{\lambda_2-\lambda_1}
  \left[\begin{array}{cc} 1 & 1\\\lambda_1&\lambda_2\end{array}\right]
  \left[\begin{array}{cc} e^{\lambda_1t} & 0\\0 & e^{\lambda_2t}\end{array}\right]
  \left[\begin{array}{cc} \lambda_2 & -1\\\ -\lambda_1&1\end{array}\right]
  \left[\begin{array}{c} y_0 \\ 0\end{array}\right]
  \nonumber\\
  &=&\frac{1}{\lambda_2-\lambda_1}
  \left[\begin{array}{cc} \lambda_2e^{\lambda_1t}-\lambda_1e^{\lambda_2t}
      & e^{\lambdaa_2t}-e^{\lambda_1t}
      \\ \lambda_1\lambda_2(e^{\lambda_1 t}-e^{\lambda_2 t}) &
      \lambda_2 e^{\lambda_2t}-\lambda_1 e^{\lambda_1t}\end{array}\right]
  \left[\begin{array}{c} y_0 \\ 0\end{array}\right]
  \nonumber\\
  &=&\frac{y_0}{\lambda_2-\lambda_1}
  \left[\begin{array}{c} \lambda_2e^{\lambda_1t}-\lambda_1e^{\lambda_2t}\\
      \lambda_1\lambda_2(e^{\lambda_1t}-e^{\lambda_2t})
    \end{array}\right]
  \nonumber
  \end{eqnarray}
  we get the same result as shown above:
  \[
  y(t)=y_1(t)=\frac{y_0}{\lambda_2-\lambda_1}(\lambda_2e^{\lambda_1t}-\lambda_1e^{\lambda_2t})
  \]

\item Nonhomogeneous sollution $x(t)=1$, i.e.,${\bf x}=[0,\;1]^T$:

  Assuming zero-initial condition $y_1(0)=y_2(0)=0$, i.e., ${\bf y}={\bf 0}$,
  the non-homogeneous solution is:
  \[
  {\bf y}(t)=e^{{\bf A}t}{\bf y}(0)+e^{{\bf A}t}\int_0^t e^{-{\bf A}\tau}{\bf x}(\tau)d\tau
  =e^{{\bf A}t}\int_0^t e^{-{\bf A}\tau} d\tau \;[0,\;1]^T
  \]

  \[
  y(t)=y_1(t)=[1,\;0]\;{\bf y}(t)=[1,\;0]\; e^{{\bf A}t}\int_0^t e^{-{\bf A}\tau} d\tau\; [0,\;1]^T
  \]
  where 
  \[
  \int_0^t e^{-{\bf A}\tau} d\tau=-{\bf A}^{-1} e^{-{\bf A}\tau}\bigg|_0^t
  ={\bf A}^{-1}( {\bf I}-e^{-{\bf A}t} )
  \]
  Substituting 
  \[
  {\bf A}^{-1}=({\bf V\Lambda V}^{-1})^{-1}={\bf V\Lambda}^{-1}{\bf V}^{-1},
  \;\;\;\;\;\;
  e^{{\bf A}t}={\bf V}e^{{\bf\Lambda}t}{\bf V}^{-1},\;\;\;\;\;\;
  e^{-{\bf A}t}={\bf V}e^{-{\bf\Lambda}t}{\bf V}^{-1}
  \]
  into the function, we get
%  \end{document}
  \begin{eqnarray}
  y(t)&=&[1,\;0]\;\left(e^{{\bf A}t}\int_0^t e^{-{\bf A}\tau} d\tau\right)\;[0,\;1]^T
  =[1,\;0]\;\left({\bf V}e^{{\bf\Lambda}t}{\bf V}^{-1}\right)\,
  \left({\bf V\Lambda}^{-1}{\bf V}^{-1}\right)
  \left({\bf I}-{\bf V}e^{-{\bf\Lambda}t}{\bf V}^{-1}\right)\;[0,\;1]^T
  \nonumber\\
  &=&[1,\;0]\;{\bf V}e^{{\bf\Lambda}t} {\bf \Lambda}^{-1}{\bf V}^{-1}
  -{\bf V}e^{{\bf\Lambda}t}{\bf\Lambda}^{-1}  e^{-{\bf\Lambda}t}{\bf V}^{-1}
  ={\bf V}e^{{\bf\Lambda}t}{\bf\Lambda}^{-1}({\bf I}-e^{-{\bf\Lambda}t} ){\bf V}^{-1}
  \;[0,\;1]^T
  \nonumber\\
  &=&[1,\;0]\;\left[\begin{array}{cc}1&1\\\lambda_1&\lambda_2\end{array}\right]
  \left[\begin{array}{cc}e^{\lambda_1t}&0\\0&e^{\lambda_2t}\end{array}\right]
  \left[\begin{array}{cc}1/\lambda_1&0\\0&1/\lambda_2\end{array}\right]
  \left[\begin{array}{cc} 1-e^{-\lambda_1t} & 0\\0 & 1-e^{-\lambda_2t}\end{array}\right]
  \frac{1}{\lambda_2-\lambda_1}
  \left[\begin{array}{cc}\lambda_2&-1\\-\lambda_1&1\end{array}\right]
  \left[\begin{array}{c}0\\1\end{array}\right]
  \nonumber\\
  &=&\left[e^{\lambda_1t},\;e^{\lambda_2t}\right]
    \left[\begin{array}{cc}1/\lambda_1&0\\0&1/\lambda_2\end{array}\right]
    \frac{1}{\lambda_2-\lambda_1}
  \left[\begin{array}{c}-(1-e^{-\lambda_1t})\\1-e^{-\lambda_2t}\end{array}\right]    
  =\frac{1}{\lambda_1\lambda_2}
  \left(1-\frac{\lambda_2e^{\lambda_1t}-\lambda_1e^{\lambda_2t}}{\lambda_2-\lambda_1}\right)
  \nonumber
  \end{eqnarray}
\end{itemize}

\end{document}


